Logic/Predicate/FirstOrder/Completeness/SearchTree.lean
@@ -1,42 +1,128 @@
-import Logic.Predicate.FirstOrder.Calculus
+import Logic.Predicate.FirstOrder.Semantics
 import Logic.Predicate.FirstOrder.Coding
+import Logic.Vorspiel.Order
 
 universe u v
 
 namespace FirstOrder
 
-namespace Derivation
-
-open SubFormula
-
 variable {L : Language.{u}}
   [∀ k, DecidableEq (L.func k)] [∀ k, DecidableEq (L.rel k)]
   [∀ k, Encodable (L.func k)] [∀ k, Encodable (L.rel k)]
 
-def decomp (s : Finset (SyntacticTerm L)) :
-  SyntacticFormula L → Finset (SyntacticFormula L) → Set (Finset $ SyntacticFormula L)
-| rel _ _,  Γ => {Γ}
-| nrel _ _, Γ => {Γ}
-| ⊤,        _ => ∅
-| ⊥,        Γ => {Γ}
-| p ⋏ q,    Γ => { insert p Γ, insert q Γ }
-| p ⋎ q,    Γ => { insert q (insert p Γ) }
-| ∀' p,     Γ => { insert (SubFormula.free p) (shifts Γ) }
-| ∃' p,     Γ => { s.image (subst · p) ∪ Γ }
+def SubFormula.index (p : SyntacticFormula L) : ℕ  := Encodable.encode p
 
-def IsTerminal (Δ : Finset (SyntacticFormula L)) : Prop :=
-  ∃ (k : ℕ) (r : L.rel k) (v : Fin k → SyntacticTerm L), rel r v ∈ Δ ∧ nrel r v ∈ Δ
+lemma SubFormula.index_inj {p q : SyntacticFormula L} : p.index = q.index ↔ p = q :=
+  Encodable.encode_inj
 
-inductive SearchTreeAux (i : ℕ) : Finset (SyntacticFormula L) → Finset (SyntacticFormula L) → Prop
-| decomp : ∀ (Γ₁ : Finset (SyntacticFormula L)) (Γ₂ : Finset (SyntacticFormula L))
-    (p : SyntacticFormula L) (hp : p ∈ Γ₁) (hi : p.index = i.unpair.fst),
-    sigma.mk m₂ Γ₂ ∈ decomp i.unpair.snd p Γ₁ → search_tree_decomp Γ₂ Γ₁
-| none : ∀ {m} (Γ : finset (bounded_formula L m)) 
-    (hi : ∀ p ∈ Γ, subformula.index p ≠ i.unpair.fst),
-    search_tree_decomp Γ Γ
+open SubFormula
 
-#check decomp
+def sequentUpper (Γ : Sequent L) : ℕ := Γ.sup SubFormula.upper
 
-end Derivation
+lemma not_fvar?_sequentUpper {p : SyntacticFormula L} {Γ : Sequent L} (h : p ∈ Γ) : ¬fvar? p (sequentUpper Γ) :=
+  not_fvar?_of_lt_upper p (by simpa[sequentUpper] using Finset.le_sup h)
+
+inductive SearchTreeAux (s : ℕ) (Γ : Sequent L) : SyntacticFormula L → Sequent L → Prop
+  | rel {k} (r : L.rel k) (v) :
+      nrel r v ∉ Γ → SearchTreeAux s Γ (rel r v) ∅ 
+  | nrel {k} (r : L.rel k) (v) :
+      rel r v ∉ Γ → SearchTreeAux s Γ (nrel r v) ∅
+  | falsum : SearchTreeAux s Γ ⊥ ∅
+  | andLeft (p q : SyntacticFormula L) : SearchTreeAux s Γ (p ⋏ q) {p}
+  | andRight (p q : SyntacticFormula L) : SearchTreeAux s Γ (p ⋏ q) {q}
+  | or (p q : SyntacticFormula L) : SearchTreeAux s Γ (p ⋎ q) {p, q}
+  | all (p : SyntacticSubFormula L 1) : SearchTreeAux s Γ (∀' p) {subst &(sequentUpper Γ) p}
+  | ex (p : SyntacticSubFormula L 1) : SearchTreeAux s Γ (∃' p) ((SubTerm.enumLt s).image (subst · p))
+
+inductive SearchTreeAt (s : ℕ) : Sequent L → Sequent L → Prop
+  | decomp (p : SyntacticFormula L) (Γ Δ : Sequent L) :
+      p.index = s.unpair.1 → p ∈ Γ → SearchTreeAux s.unpair.2 Γ p Δ → SearchTreeAt s (Δ ∪ Γ) Γ
+  | refl (Γ : Sequent L) : (∀ p ∈ Γ, p.index ≠ s.unpair.1) → SearchTreeAt s Γ Γ
+
+local notation:25 Γ₁" ≺[" s:25 "] " Γ₂:80 => SearchTreeAt s Γ₁ Γ₂
+
+lemma searchtreeAt_iff_decomp_of_index {Γ' Γ : Sequent L} {p} (hp : p ∈ Γ) (hs : index p = s.unpair.1) :
+  Γ' ≺[s] Γ ↔ ∃ Δ, SearchTreeAux s.unpair.2 Γ p Δ ∧ Γ' = Δ ∪ Γ :=
+  ⟨by rintro (_ | _)
+      case decomp q E hs' hq h =>
+        have : p = q := SubFormula.index_inj.mp (by simp[hs, hs'])
+        exact ⟨E, by simpa[this] using h, rfl⟩
+      case refl H =>
+        have := H p hp; contradiction,
+   by rintro ⟨Δ, h, rfl⟩; exact SearchTreeAt.decomp p Γ Δ hs hp h⟩
+
+inductive SearchTree.IsUnder (Γ : Sequent L) : ℕ × Sequent L → Prop
+  | top : SearchTree.IsUnder Γ (0, Γ)
+  | lt {s} {Γ₁ Γ₂ : Sequent L} : Γ₂ ≺[s] Γ₁ → SearchTree.IsUnder Γ (s, Γ₁) → SearchTree.IsUnder Γ (s + 1, Γ₂)
+
+def SearchTreeUnder (Γ : Sequent L) := {p // SearchTree.IsUnder Γ p}
+
+inductive SearchTree (Γ : Sequent L) : SearchTreeUnder Γ → SearchTreeUnder Γ → Prop
+  | intro {s : ℕ} {Δ₁ Δ₂ : Sequent L} {h₁ : SearchTree.IsUnder Γ (s, Δ₁)} {h₂ : SearchTree.IsUnder Γ (s + 1, Δ₂)} :
+      Δ₂ ≺[s] Δ₁ → SearchTree Γ ⟨(s + 1, Δ₂), h₂⟩ ⟨(s, Δ₁), h₁⟩
+
+namespace SearchTree
+
+section WellFounded
+
+variable {Γ : Sequent L} (wf : WellFounded (SearchTree Γ))
+
+noncomputable def SearchTree.recursion {C : SearchTreeUnder Γ → Sort _} 
+  (τ) (h : ∀ τ₁, (∀ τ₂, SearchTree Γ τ₂ τ₁ → C τ₂) → C τ₁) : C τ :=
+  WellFounded.recursion wf τ h
+
+noncomputable def syntacticMainLemmaAux (τ : SearchTreeUnder Γ) : ⊩ τ.val.2 := by
+  apply SearchTree.recursion wf τ
+  intro ⟨⟨s, Δ⟩, hΔ⟩ ih; simp
+  have ih : ∀ Δ₂ : Sequent L, Δ₂ ≺[s] Δ → ⊩ Δ₂ :=
+    fun Δ₂ h => ih ⟨(s + 1, Δ₂), SearchTree.IsUnder.lt h hΔ⟩ (SearchTree.intro h)
+  by_cases hs : ∀ p ∈ Δ, p.index ≠ s.unpair.fst
+  case pos =>
+    exact ih Δ (SearchTreeAt.refl Δ hs)
+  case neg =>
+    have : ∃ p ∈ Δ, index p = s.unpair.1 := by simpa using hs
+    choose p hp using this
+    cases p using cases'
+    case hverum =>
+      exact Derivation.verum Δ hp.1
+    case hfalsum =>
+      have : Δ ≺[s] Δ := (searchtreeAt_iff_decomp_of_index hp.1 hp.2).mpr ⟨∅, SearchTreeAux.falsum, by simp⟩
+      exact ih Δ this
+    case hrel k r v =>
+      by_cases hrv : nrel r v ∈ Δ
+      · exact Derivation.axL Δ r v hp.1 hrv
+      · have : Δ ≺[s] Δ := (searchtreeAt_iff_decomp_of_index hp.1 hp.2).mpr ⟨∅, SearchTreeAux.rel r v hrv, by simp⟩
+        exact ih Δ this
+    case hnrel k r v =>
+      by_cases hrv : rel r v ∈ Δ
+      · exact Derivation.axL Δ r v hrv hp.1
+      · have : Δ ≺[s] Δ := (searchtreeAt_iff_decomp_of_index hp.1 hp.2).mpr ⟨∅, SearchTreeAux.nrel r v hrv, by simp⟩
+        exact ih Δ this
+    case hand p q =>
+      have dp : insert p Δ ≺[s] Δ := (searchtreeAt_iff_decomp_of_index hp.1 hp.2).mpr ⟨_, SearchTreeAux.andLeft p q, rfl⟩
+      have dq : insert q Δ ≺[s] Δ := (searchtreeAt_iff_decomp_of_index hp.1 hp.2).mpr ⟨_, SearchTreeAux.andRight p q, rfl⟩
+      have : ⊩ insert (p ⋏ q) Δ := Derivation.and Δ p q (ih _ dp) (ih _ dq)
+      exact this.cast (by simp[hp.1])
+    case hor p q =>
+      have : {p, q} ∪ Δ ≺[s] Δ := (searchtreeAt_iff_decomp_of_index hp.1 hp.2).mpr ⟨_, SearchTreeAux.or p q, rfl⟩
+      have : ⊩ insert (p ⋎ q) Δ := Derivation.or ((ih _ this).cast (by simp[Finset.insert_eq]))
+      exact this.cast (by simp[hp.1])
+    case hall p =>
+      have : {subst &(sequentUpper Δ) p} ∪ Δ ≺[s] Δ := (searchtreeAt_iff_decomp_of_index hp.1 hp.2).mpr ⟨_, SearchTreeAux.all p, rfl⟩
+      have : ⊩ insert (subst &(sequentUpper Δ) p) Δ := ih _ this
+      have : ⊩ insert (∀' p) Δ := Derivation.genelalizeByNewver (not_fvar?_sequentUpper hp.1) (fun _ hq => not_fvar?_sequentUpper hq) this
+      exact this.cast (by simp[hp.1])
+    case hex p =>
+      have : ((SubTerm.enumLt s.unpair.2).image (subst · p)) ∪ Δ ≺[s] Δ :=
+        (searchtreeAt_iff_decomp_of_index hp.1 hp.2).mpr ⟨_, SearchTreeAux.ex p, rfl⟩
+      have : ⊩ ((SubTerm.enumLt s.unpair.2).image (subst · p)) ∪ Δ := ih _ this
+      have : ⊩ insert (∃' p) Δ := Derivation.exOfInstances (SubTerm.enumLtList s.unpair.2) p (by simpa[List.toFinset_map] using this)
+      exact this.cast (by simp[hp.1])  
+    
+noncomputable def syntacticMainLemma : ⊩ Γ := syntacticMainLemmaAux wf ⟨(0, Γ), SearchTree.IsUnder.top (Γ := Γ)⟩
+
+end WellFounded
+
+end SearchTree
 
 end FirstOrder
